theories/logrel/logrel.v
@@ -31,7 +31,7 @@ Section logrel.
       full entries.
       Pagetable entries are transferred along as both sender and receiver could be the exclusive owner of those pages. *)
   Definition transaction_pagetable_entries_transferred i (trans: gmap Addr transaction) : iProp Σ:=
-    big_sepFM trans (λ kv, (kv.2.1.1.1.1 = i ∨ kv.2.1.1.1.2 = i) ∧ kv.2.1.2 = Donation ) (λ k v, k -{1/4}>t v.1 ∗ pgt_1_4 v.1.1.2 v.1.1.1.1 true)%I.
+    big_sepFM trans (λ kv, (kv.2.1.1.1.1 = i ∨ kv.2.1.1.1.2 = i) ∧ kv.2.1.2 = Donation) (λ k v, k -{1/4}>t v.1 ∗ pgt_1_4 v.1.1.2 v.1.1.1.1 true)%I.
 
   (* [retrieval entries]: half of all retrieval entries of i-related transactions are required.
      For transactions where i is the sender, we need the corresponding retrieval entries to check if it is allowed for i to reclaim,
